\begin{homeworkProblem}
  Mostrar que:
  \begin{solution}
    \begin{enumerate}
      \item $sin(3x)=3cos^2(x)sin(x)-sin^3(x)$.\\
        Note que:
        \begin{align*}
          sin(3x)&=Ima(cos(3x)+isen(3x))\\
          &=Ima(e^{i3x})\\
          &=Ima([e^{ix}]^3)\\
          &=Ima([cos(x)+isen(x)]^3)\\
          &=Ima(cos^3(x) + 3icos^2(x)sin(x) - 3cos(x)sin^2(x) - isin^3(x))\\
          &=3cos^2(x)sin(x)-sin^3(x)
        \end{align*}
      \item $cos(3x)=cos^3(x)-3cos(x)sin^2(x)$.\\
        Note que utilizando la expresi√≥n compleja del punto anterior se tiene que:
        \begin{align*}
          cos(3x)&=Re(cos(3x)+isen(3x))\\
          &=Re(cos^3(x) + 3icos^2(x)sin(x) - 3cos(x)sin^2(x) - isin^3(x))\\
          &=cos^3(x)-3cos(x)sin^2(x)
        \end{align*}
      \item $cos(8x)+28cos(4x)+35=64(cos^8(x)+sin^8(x))$.\\
      Note que:
      \begin{align*}
        (e^{ix}+e^{-ix})^{8}+(e^{ix}-e^{-ix})^{8}&=2(e^{i8x} + e^{-i8x})+ 56(e^{4ix} + e^{-4ix}) + 140,
      \end{align*}
      es decir:
      \begin{align*}
        (2cos(x))^{8}+(2sin(x))^{8}&= 2(2cos(8x)) + 56(2cos(4x)) + 140
      \end{align*}
      lo que implica:
      \begin{align*}
        64(cos^{8}(x)+sin^{8}(x))&=cos(8x)+28cos(4x)+35
      \end{align*}
    \end{enumerate}
  \end{solution}
\end{homeworkProblem}
