\begin{homeworkProblem}
  Para $k$ entero positivo, sea $J_k(z) = \sum_{0}^{\infty} \frac{(-1)^n}{n! (n+k)!} \left( \frac{z}{2} \right)^{2n+k}$. Probar:
  \begin{align*}
    z^2 J_k''(z) + zJ_k'(z) + (z^2 - k^2) J_k(z) = 0.   
  \end{align*}
  \begin{solution}
    Dada la función:
    \begin{align*}
      J_k(z) &= \sum_{n=0}^{\infty} \frac{(-1)^n}{n! (n+k)!} \left( \frac{z}{2} \right)^{2n+k},
    \end{align*}
    calculamos sus derivadas y productos:
    \begin{align*}
      zJ_k'(z) &= \sum_{n=0}^{\infty} \frac{(-1)^n}{n! (n+k)!} (2n+k)\left( \frac{z}{2} \right)^{2n+k} \\
      z^2J_k''(z) &= \sum_{n=0}^{\infty} \frac{(-1)^n}{n! (n+k)!} \cdot (2n+k)(2n+k-1) \left( \frac{z}{2} \right)^{2n+k}.
    \end{align*}
    Sustituyendo en la ecuación:
    \begin{align*}
      z^2 J_k''(z) + z J_k'(z) + (z^2 - k^2) J_k(z),
    \end{align*}
    obtenemos:
  \end{solution}
\end{homeworkProblem}
